Using records for partial functions

IndexFunctions.v
@@ -43,34 +43,31 @@ Global Instance index_map_equiv {domain range:nat}:
   :=
     fun f g => forall (x:nat) (xd: x<domain), ⟦ f ⟧ x = ⟦ g ⟧ x.
 
-
 Section Inversions.
-  Definition partial_function_def domain range f' :=
-    forall x, x<range -> forall z, (((f' x) ≡ Some z) -> z < domain).
+
+  Record partial_index_map (domain range : nat)
+    :=
+      PartialIndexMap { partial_index_f : nat -> option nat; partial_index_f_spec :  forall x, x<domain -> forall z, (((partial_index_f x) ≡ Some z) -> z < range)}.
   
-  Definition inverse_map_spec (i o: nat) :=
-    { f': nat -> option nat | partial_function_def i o f'}.
-  
-  Program Definition build_inverse_map_spec
+  Program Definition build_inverse_index_map
           {i o: nat}
-          (f: index_map i o): inverse_map_spec i o
-    := fun y =>
-         List.fold_right
-           (fun x' p => if eq_nat_dec y ( ⟦ f ⟧ x') then Some x' else p)
-           None
-           (rev_natrange_list i).
+          (f: index_map i o): partial_index_map o i
+    := PartialIndexMap o i (fun y =>
+                              List.fold_right
+                                (fun x' p => if eq_nat_dec y ( ⟦ f ⟧ x') then Some x' else p)
+                                None
+                                (rev_natrange_list i)) _.
   Next Obligation.
     destruct f.  simpl.
-    unfold partial_function_def.
     intros.
     induction i.
     crush.
     simpl in H0.
     destruct (eq_nat_dec x (index_f0 i)); crush.
   Defined.
+  
 End Inversions.
   
-
 Section Permutations.
   Fixpoint natrange_f_spec
            (n:nat)
